Trying to untangle invariants of the stack injection for the raww asm and inlining to go through

common/Memimpl.v
@@ -862,7 +862,8 @@ Record extends' {injperm: InjectPerm} (m1 m2: mem) : Prop :=
     mext_inj:  mem_inj inject_id (flat_frameinj (length (stack_adt m1))) m1 m2;
     mext_perm_inv: forall b ofs k p,
       perm m2 b ofs k p ->
-      perm m1 b ofs k p \/ ~perm m1 b ofs Max Nonempty
+      perm m1 b ofs k p \/ ~perm m1 b ofs Max Nonempty;
+    mext_same_length: length (stack_adt m1) = length (stack_adt m2);
   }.
 
 Definition extends {injperm: InjectPerm} := extends'.
@@ -946,13 +947,8 @@ Record magree' {injperm: InjectPerm} (m1 m2: mem) (P: locset) : Prop := mk_magre
     nextblock m2 = nextblock m1;
   ma_stack_adt:
     stack_inject inject_id (flat_frameinj (length (stack_adt m1))) (perm m1) (stack_adt m1) (stack_adt m2);
-  (* ma_not_in_any_frame: *)
-  (*   list_forall2 *)
-  (*       (fun x y => *)
-  (*          forall b, *)
-  (*            in_frame (fst x) b -> (fst y) = None -> *)
-  (*            ~ in_frames (stack_adt m2) b *)
-  (*       ) (stack_adt m1) (stack_adt m2) *)
+  ma_same_length:
+    length (stack_adt m1) = length (stack_adt m2);
 }.
 
 Definition magree {injperm: InjectPerm} := magree'.
@@ -3769,7 +3765,8 @@ Lemma is_stack_top_inj:
   forall f g m1 m2 b1 b2 delta
     (MINJ: mem_inj f g m1 m2)
     (FB: f b1 = Some (b2, delta))
-    (IST: is_stack_top (stack_adt m1) b1),
+    (IST: is_stack_top (stack_adt m1) b1)
+    (G0: frameinj_pack_after O g),
     is_stack_top (stack_adt m2) b2.
 Proof.
   intros. inv MINJ.
@@ -3783,21 +3780,22 @@ Lemma is_stack_top_extends:
     is_stack_top (stack_adt m2) b.
 Proof.
   intros.
-  eapply is_stack_top_inj; eauto. inv MINJ; eauto. reflexivity.
+  inv MINJ.
+  eapply is_stack_top_inj; eauto. reflexivity.
+  unfold flat_frameinj. red; intros. destr_in H0. inv H0; omega.
 Qed.
 
 Lemma is_stack_top_inject:
   forall f g m1 m2 b1 b2 delta
     (MINJ: inject f g m1 m2)
     (FB: f b1 = Some (b2, delta))
+    (G0: frameinj_pack_after O g)
     (IST: is_stack_top (stack_adt m1) b1),
     is_stack_top (stack_adt m2) b2.
 Proof.
   intros.
   eapply is_stack_top_inj; eauto. inv MINJ; eauto.
 Qed.
-
-
 
 Lemma get_frame_info_inj:
   forall f g m1 m2 b1 b2 delta
@@ -3846,12 +3844,11 @@ Proof.
   omega.
 Qed.
 
-
-
 Lemma stack_access_inj:
   forall f g m1 m2 b1 b2 delta lo hi p
     (MINJ : mem_inj f g m1 m2)
     (FB : f b1 = Some (b2, delta))
+    (G0: frameinj_pack_after O g)
     (RP: range_perm m1 b1 lo hi Cur p)
     (IPC: inject_perm_condition p)
     (NPSA: stack_access (stack_adt m1) b1 lo hi),
@@ -3874,11 +3871,12 @@ Lemma valid_access_inj_gen:
              range_perm m1 b1 ofs (ofs+size_chunk chunk) Max p ->
              (align_chunk chunk | delta)),
     f b1 = Some(b2, delta) ->
+    (perm_order p Writable ->       frameinj_pack_after O g) ->
     valid_access m1 chunk b1 ofs p ->
     inject_perm_condition p ->
     valid_access m2 chunk b2 (ofs + delta) p.
 Proof.
-  intros. destruct H0 as (A & B & C). split; [| split].
+  intros. destruct H1 as (A & B & C). split; [| split].
   - replace (ofs + delta + size_chunk chunk)
       with ((ofs + size_chunk chunk) + delta) by omega.
     red; intros.
@@ -3893,11 +3891,11 @@ Proof.
     eapply stack_access_inj_gen; eauto.
 Qed.
 
-
 Lemma valid_access_inj:
   forall f g m1 m2 b1 b2 delta chunk ofs p,
   mem_inj f g m1 m2 ->
   f b1 = Some(b2, delta) ->
+  (perm_order p Writable -> frameinj_pack_after O g) ->
   valid_access m1 chunk b1 ofs p ->
   inject_perm_condition p ->
   valid_access m2 chunk b2 (ofs + delta) p.
@@ -3939,6 +3937,7 @@ Proof.
   exists (decode_val chunk (getN (size_chunk_nat chunk) (ofs + delta) (m2.(mem_contents)#b2))).
   split. unfold load. apply pred_dec_true.
   eapply valid_access_inj; eauto with mem.
+  inversion 1.
   eapply inject_perm_condition_writable; constructor.
   exploit load_result; eauto. intro. rewrite H2.
   apply decode_val_inject. eapply getN_inj; eauto.
@@ -4001,6 +4000,7 @@ Lemma store_mapped_inj:
     store chunk m1 b1 ofs v1 = Some n1 ->
     meminj_no_overlap f m1 ->
     f b1 = Some (b2, delta) ->
+    frameinj_pack_after O g ->
     Val.inject f v1 v2 ->
     exists n2,
       store chunk m2 b2 (ofs + delta) v2 = Some n2
@@ -4012,7 +4012,7 @@ Proof.
     eapply valid_access_inj; eauto with mem.
     eapply inject_perm_condition_writable; constructor.
   }
-  destruct (valid_access_store' _ _ _ _ v2 H4) as [n2 STORE].
+  destruct (valid_access_store' _ _ _ _ v2 H5) as [n2 STORE].
   exists n2; split. auto.
   constructor.
   - (* perm *)
@@ -4042,7 +4042,7 @@ Proof.
         eapply H1; eauto. eauto 6 with mem.
         exploit store_valid_access_3. eexact H0. intros [A B].
         eapply perm_implies. apply perm_cur_max. apply A. omega. auto with mem.
-        destruct H8. congruence. omega.
+        destruct H9. congruence. omega.
       * (* block <> b1, block <> b2 *)
         eapply mi_memval; eauto. eauto with mem.
   - rewrite (store_stack_adt _ _ _ _ _ _ STORE).
@@ -4112,12 +4112,14 @@ Lemma storebytes_mapped_inj:
     storebytes m1 b1 ofs bytes1 = Some n1 ->
     meminj_no_overlap f m1 ->
     f b1 = Some (b2, delta) ->
+    frameinj_pack_after O g ->
     list_forall2 (memval_inject f) bytes1 bytes2 ->
     exists n2,
       storebytes m2 b2 (ofs + delta) bytes2 = Some n2
       /\ mem_inj f g n1 n2.
 Proof.
-  intros. inversion H.
+  intros f g m1 b1 ofs bytes1 n1 m2 b2 delta bytes2 H H0 H1 H2 G0 H3.
+  inversion H.
   assert (range_perm m2 b2 (ofs + delta) (ofs + delta + Z_of_nat (length bytes2)) Cur Writable).
   {
     replace (ofs + delta + Z_of_nat (length bytes2))
@@ -4567,8 +4569,7 @@ Proof.
   - inversion 1; eauto. intros; exfalso; apply H0. eapply in_frames_in_frame; eauto.
   - intros i j H; destr_in H; inv H.
   - intros. exists i; destr.
-  - intros. exists j; destr.
-  - intros i j H; destr_in H; inv H. omega.
+  (* - intros i j H; destr_in H; inv H. omega. *)
   - intros i1 i2 f1 f2 FAP1 FAP2 H; repeat destr_in H.
     assert (f1 = f2) by (eapply frame_at_same_pos; eauto). subst. auto.
 Qed.
@@ -4582,6 +4583,7 @@ Proof.
   intros. unfold inject_id in H; inv H. replace (ofs + 0) with ofs by omega.
   apply memval_lessdef_refl.
   apply stack_inject_id. auto.
+  auto.
 Qed.
 
 Theorem load_extends:
@@ -4619,6 +4621,31 @@ Proof.
   replace ofs with (ofs + 0) by omega. eapply loadbytes_inj; eauto.
 Qed.
 
+Lemma storev_stack_adt:
+  forall chunk m1 addr v m2,
+    storev chunk m1 addr v = Some m2 ->
+    stack_adt m2 = stack_adt m1.
+Proof.
+  intros chunk m1 addr v m2 H; unfold storev in H; destr_in H.
+  eapply store_stack_adt; eauto.
+Qed.
+
+Ltac rewrite_stack_backwards :=
+  repeat match goal with
+  | H: store _ ?m1 _ _ _ = Some ?m2 |- context [stack_adt ?m2] =>
+    rewrite (store_stack_adt _ _ _ _ _ _ H)
+  | H: storev _ ?m1 _ _ = Some ?m2 |- context [stack_adt ?m2] =>
+    rewrite (storev_stack_adt _ _ _ _ _ H)
+  | H: storebytes ?m1 _ _ _ = Some ?m2 |- context [stack_adt ?m2] =>
+    rewrite (storebytes_stack_adt _ _ _ _ _ H)
+  | H: alloc ?m1 _ _ = (?m2,_) |- context [stack_adt ?m2] =>
+    rewrite (alloc_stack_adt _ _ _ _ _ H)
+  | H: free ?m1 _ _ _ = Some ?m2 |- context [stack_adt ?m2] =>
+    rewrite (free_stack_adt _ _ _ _ _ H)
+  | H: drop_perm ?m1 _ _ _ _ = Some ?m2 |- context [stack_adt ?m2] =>
+    rewrite (drop_perm_stack_adt _ _ _ _ _ _ H)
+  end.
+
 Theorem store_within_extends:
   forall chunk m1 m2 b ofs v1 m1' v2,
   extends m1 m2 ->
@@ -4632,6 +4659,7 @@ Proof.
   exploit store_mapped_inj; eauto.
     unfold inject_id; red; intros. inv H3; inv H4. auto.
     unfold inject_id; reflexivity.
+    unfold flat_frameinj. red; intros. destr_in H3. inv H3; omega.
     rewrite val_inject_id. eauto.
   intros [m2' [A B]].
   exists m2'; split.
@@ -4642,6 +4670,7 @@ Proof.
   auto.
   erewrite store_stack_adt; eauto.
   intros. exploit mext_perm_inv0; intuition eauto using perm_store_1, perm_store_2.
+  rewrite_stack_backwards. auto.
 Qed.
 
 Theorem store_outside_extends:
@@ -4655,7 +4684,8 @@ Proof.
   rewrite (nextblock_store _ _ _ _ _ _ H0). auto.
   eapply store_outside_inj; eauto.
   unfold inject_id; intros. inv H2. eapply H1; eauto. omega.
-  intros. eauto using perm_store_2. 
+  intros. eauto using perm_store_2.
+  rewrite_stack_backwards. auto.
 Qed.
 
 Theorem storev_extends:
@@ -4686,6 +4716,7 @@ Proof.
   exploit storebytes_mapped_inj; eauto.
     unfold inject_id; red; intros. inv H3; inv H4. auto.
     unfold inject_id; reflexivity.
+    unfold flat_frameinj; red; intros. repeat destr_in H3; omega.
   intros [m2' [A B]].
   exists m2'; split.
   replace (ofs + 0) with ofs in A by omega. auto.
@@ -4695,6 +4726,7 @@ Proof.
   auto.
   erewrite storebytes_stack_adt; eauto.
   intros. exploit mext_perm_inv0; intuition eauto using perm_storebytes_1, perm_storebytes_2.
+  rewrite_stack_backwards. auto.
 Qed.
 
 Theorem storebytes_outside_extends:
@@ -4709,6 +4741,7 @@ Proof.
   eapply storebytes_outside_inj; eauto.
   unfold inject_id; intros. inv H2. eapply H1; eauto. omega.
   intros. eauto using perm_storebytes_2. 
+  rewrite_stack_backwards. auto.
 Qed.
 
 Theorem alloc_extends:
@@ -4755,6 +4788,7 @@ Proof.
     left. apply perm_implies with Freeable; auto with mem. eapply perm_alloc_2; eauto.
     right; tauto.
     exploit mext_perm_inv0; intuition eauto using perm_alloc_1, perm_alloc_4.
+  -   rewrite_stack_backwards. auto.
 Qed.
 
 Theorem free_left_extends:
@@ -4771,6 +4805,7 @@ Proof.
   eapply perm_free_inv in A; eauto. destruct A as [[A B]|A]; auto.
   subst b0. right; eapply perm_free_2; eauto.
   intuition eauto using perm_free_3.
+  rewrite_stack_backwards. auto.
 Qed.
 
 Theorem free_right_extends:
@@ -4785,6 +4820,7 @@ Proof.
   eapply free_right_inj; eauto.
   unfold inject_id; intros. inv H. eapply H1; eauto. omega.
   intros. eauto using perm_free_3. 
+  rewrite_stack_backwards. auto.
 Qed.
 
 Theorem free_parallel_extends:
@@ -4815,6 +4851,7 @@ Proof.
   eapply perm_free_inv in A; eauto. destruct A as [[A B]|A]; auto.
   subst b0. right; eapply perm_free_2; eauto.
   right; intuition eauto using perm_free_3.
+  rewrite_stack_backwards. auto.
 Qed.
 
 Theorem valid_block_extends:
@@ -4839,6 +4876,16 @@ Theorem perm_extends_inv:
 Proof.
   intros. inv H; eauto.
 Qed.
+
+Lemma flat_frameinj_pack:
+  forall x n,
+    frameinj_pack_after x (flat_frameinj n).
+Proof.
+  unfold flat_frameinj. red; intros.
+  repeat destr_in H0; omega.
+Qed.
+
+Hint Resolve flat_frameinj_pack.
 
 Theorem valid_access_extends:
   forall m1 m2 chunk b ofs p,
@@ -4887,6 +4934,7 @@ Proof.
   rewrite Zplus_0_r. auto.
 - auto.
 - auto.
+-   rewrite_stack_backwards. auto.
 Qed.
 
 Lemma magree_extends:
@@ -5050,6 +5098,7 @@ Proof.
   2: eapply ma_stack_adt; eauto.
   inversion 1.
   eapply perm_storebytes_2; eauto.
+- inv H; rewrite_stack_backwards. auto.
 Qed.
 
 Lemma magree_storebytes_left:
@@ -5076,6 +5125,7 @@ Proof.
   2: eapply ma_stack_adt; eauto.
   unfold inject_id. intros b0 ofs0 k p b' delta H3 H4. inv H3.
   eapply perm_storebytes_2; eauto.
+- inv H; rewrite_stack_backwards. auto.
 Qed.
 
 Lemma magree_store_left:
@@ -5131,6 +5181,7 @@ Proof.
   2: eapply ma_stack_adt; eauto.
   unfold inject_id. intros b0 ofs0 k p b' delta H3 H4. inv H3.
   eapply perm_free_3; eauto.
+- inv MAGREE; rewrite_stack_backwards. auto.
 Qed.
 
 Lemma magree_valid_access:
@@ -5206,6 +5257,7 @@ Theorem valid_access_inject:
   f b1 = Some(b2, delta) ->
   inject f g m1 m2 ->
   valid_access m1 chunk b1 ofs p ->
+  (perm_order p Writable -> frameinj_pack_after O g) ->
   inject_perm_condition p ->
   valid_access m2 chunk b2 (ofs + delta) p.
 Proof.
@@ -5222,7 +5274,7 @@ Proof.
   intros.
   rewrite valid_pointer_valid_access in H1.
   rewrite valid_pointer_valid_access.
-  eapply valid_access_inject; eauto.
+  eapply valid_access_inject; eauto. inversion 1.
   eapply inject_perm_condition_writable; constructor.
 Qed.
 
@@ -5424,7 +5476,7 @@ Proof.
   assert (valid_access m chunk b ofs Nonempty).
     split. red; intros; apply H3. omega. split. congruence.
     inversion 1.
-    exploit valid_access_inject; eauto.
+    exploit valid_access_inject; eauto. inversion 1.
     eapply inject_perm_condition_writable; constructor.
     unfold valid_access. intros (C & D & E).
     congruence.
@@ -5475,6 +5527,7 @@ Theorem store_mapped_inject:
   inject f g m1 m2 ->
   store chunk m1 b1 ofs v1 = Some n1 ->
   f b1 = Some (b2, delta) ->
+  frameinj_pack_after O g ->
   Val.inject f v1 v2 ->
   exists n2,
     store chunk m2 b2 (ofs + delta) v2 = Some n2
@@ -5558,6 +5611,7 @@ Theorem storev_mapped_inject:
   storev chunk m1 a1 v1 = Some n1 ->
   Val.inject f a1 a2 ->
   Val.inject f v1 v2 ->
+  frameinj_pack_after O g ->
   exists n2,
     storev chunk m2 a2 v2 = Some n2 /\ inject f g n1 n2.
 Proof.
@@ -5574,12 +5628,14 @@ Theorem storebytes_mapped_inject:
   inject f g m1 m2 ->
   storebytes m1 b1 ofs bytes1 = Some n1 ->
   f b1 = Some (b2, delta) ->
+  frameinj_pack_after O g ->
   list_forall2 (memval_inject f) bytes1 bytes2 ->
   exists n2,
     storebytes m2 b2 (ofs + delta) bytes2 = Some n2
     /\ inject f g n1 n2.
 Proof.
-  intros. inversion H.
+  intros f g m1 b1 ofs bytes1 n1 m2 b2 delta bytes2 H H0 H1 FPA H2.
+  inversion H.
   exploit storebytes_mapped_inj; eauto. intros [n2 [STORE MI]].
   exists n2; split. eauto. constructor.
 (* inj *)
@@ -6301,78 +6357,20 @@ Proof.
       exfalso; apply H3. eapply in_frames_in_frame; eauto.
     * intros i j A; destr_in A.
     * intros; exists i; destr.
-    * intros; exists j; destr.
-    * intros i j A; repeat destr_in A. omega.
+    (* * intros i j A; repeat destr_in A. omega. *)
     * intros i1 i2 f1 f2 FAP1 FAP2 A; repeat destr_in A.
       assert (f1=f2) by (eapply frame_at_same_pos; eauto). subst. auto.
 Qed.
 
 (** Composing two memory injections. *)
 
-(* Lemma not_in_frames_frame_inject: *)
-(*   forall b b' delta f (FB: f b = Some (b', delta)) m1 l l0, list_forall2 (option_frame_inject f g m1) l l0 -> ~ in_frames l b -> ~ in_frames l0 b'. *)
-(* Proof. *)
-(*   induction 2; simpl; intros; eauto.  *)
-(*   destruct a1, b1; simpl in *; subst; eauto. *)
-(*   intuition. *)
-(*   unfold option_frame_inject in H. simpl in H. *)
-(*   repeat destr_in H. *)
-(*   inv H5; simpl in *; intros; eauto; autospe; intuition try congruence. *)
-(* Qed. *)
-
-(* Lemma not_in_frames_mem_inj: *)
-(*    forall f g m1 m2 b b' delta, *)
-(*      f b = Some (b', delta) -> *)
-(*      mem_inj f g m1 m2 -> *)
-(*      ~ in_frames ( (stack_adt m1)) b -> *)
-(*      ~ in_frames ( (stack_adt m2)) b'. *)
-(* Proof. *)
-(*   destruct 2.  *)
-(*   eapply not_in_frames_frame_inject; eauto.   *)
-(* Qed. *)
-
-(* Lemma not_in_frames_extends: *)
-(*    forall m1 m2 b, *)
-(*      extends m1 m2 -> *)
-(*      ~ in_frames ((stack_adt m1)) b -> *)
-(*      ~ in_frames ((stack_adt m2)) b. *)
-(* Proof. *)
-(*   destruct 1. destruct mext_inj0. *)
-(*   eapply not_in_frames_frame_inject; eauto. *)
-(*   reflexivity. *)
-(* Qed. *)
-
-(* Lemma not_in_frames_inject: *)
-(*    forall f g m1 m2 b b' delta, *)
-(*      f b = Some (b', delta) -> *)
-(*      inject f g m1 m2 -> *)
-(*      ~ in_frames ( (stack_adt m1)) b -> *)
-(*      ~ in_frames ( (stack_adt m2)) b'. *)
-(* Proof. *)
-(*   destruct 2. destruct mi_inj0. *)
-(*   eapply not_in_frames_frame_inject; eauto.   *)
-(* Qed. *)
-
-
-(* Lemma frame_inject_in_frame: *)
-(*   forall f g m f1 f2, *)
-(*     match f1, f2 with *)
-(*       Some f1, Some f2 => frame_inject _ f g m f1 f2 *)
-(*     | _, _ => False *)
-(*     end -> *)
-(*     forall b b' delta, *)
-(*       f b = Some (b', delta) -> *)
-(*       in_frame f1 b -> in_frame f2 b'. *)
-(* Proof. *)
-(*   destruct f1, f2; simpl; intros; intuition.  *)
-(*   inv H; simpl; intros; autospe; intuition. *)
-(* Qed. *)
-
 Lemma mem_inj_compose:
   forall f f' g g' m1 m2 m3,
-  mem_inj f g m1 m2 -> mem_inj f' g' m2 m3 -> mem_inj (compose_meminj f f') (compose_frameinj g g') m1 m3.
+    frameinj_surjective g (length (stack_adt m2)) ->
+    mem_inj f g m1 m2 -> mem_inj f' g' m2 m3 -> mem_inj (compose_meminj f f') (compose_frameinj g g') m1 m3.
 Proof.
-  intros. unfold compose_meminj. inv H; inv H0; constructor.
+  intros f f' g g' m1 m2 m3 SURJ H H0.
+  unfold compose_meminj. inv H; inv H0; constructor.
   - (* perm *)
     intros b1 b2 delta ofs k p CINJ PERM IPC.
     destruct (f b1) as [[b' delta'] |] eqn:?; try discriminate.
@@ -6405,9 +6403,11 @@ Qed.
 
 Theorem inject_compose:
   forall f f' g g' m1 m2 m3,
-  inject f g m1 m2 -> inject f' g' m2 m3 ->
-  inject (compose_meminj f f') (compose_frameinj g g') m1 m3.
+    frameinj_surjective g (length (stack_adt m2)) ->
+    inject f g m1 m2 -> inject f' g' m2 m3 ->
+    inject (compose_meminj f f') (compose_frameinj g g') m1 m3.
 Proof.
+  intros f f' g g' m1 m2 m3 SURJ H H0.
   unfold compose_meminj; intros.
   inv H; inv H0. constructor.
 (* inj *)
@@ -6491,17 +6491,30 @@ Proof.
   omega.
 Qed.
 
-Lemma extends_same_length_stack:
-  forall m1 m2,
-    extends m1 m2 ->
-    length (stack_adt m1) = length (stack_adt m2).
+Lemma surj_flat: forall n, frameinj_surjective (flat_frameinj n) n.
 Proof.
-  intros m1 m2 H; inv H. inv mext_inj0. inv mi_stack_blocks0.
-  apply lt_lt_eq. split; intros.
-  generalize (stack_inject_range i i). intro A; trim A. unfold flat_frameinj. destr.
-  omega.
-  destruct (stack_inject_exists_r i). auto. unfold flat_frameinj in H0; destr_in H0.
+  red; intros.
+  unfold flat_frameinj.
+  exists j; destr.
 Qed.
+
+(* Lemma extends_same_length_stack: *)
+(*   forall m1 m2, *)
+(*     extends m1 m2 -> *)
+(*     length (stack_adt m1) = length (stack_adt m2). *)
+(* Proof. *)
+(*   intros m1 m2 H; inv H. inv mext_inj0. inv mi_stack_blocks0. *)
+(*   apply lt_lt_eq. split; intros. *)
+(*   - generalize (stack_inject_range i i). intro A; trim A. unfold flat_frameinj. destr. *)
+(*     omega. *)
+(*   - destruct (lt_dec i (length (stack_adt m1))); auto. *)
+(*     destruct (lt_dec (length (stack_adt m1)) (length (stack_adt m2))). 2: omega. *)
+(*     exfalso. *)
+(*     eapply stack_inject_range. *)
+(*     unfold flat_frameinj. destr; eauto. *)
+(*     edestruct surj_flat. apply H. *)
+(*     unfold flat_frameinj in H0; destr_in H0. *)
+(* Qed. *)
 
 Lemma extends_inject_compose:
   forall f g m1 m2 m3,
@@ -6513,12 +6526,15 @@ Proof.
   replace g with (compose_frameinj (flat_frameinj (length (stack_adt m1))) g).
   eapply mem_inj_compose; eauto.
   {
+    rewrite mext_same_length0. apply surj_flat.
+  }
+  {
     apply extensionality. unfold compose_frameinj. intros.
     unfold flat_frameinj. destruct lt_dec. auto.
     destruct (g x) eqn:GX; auto.
     inv mi_inj0.
     eapply stack_inject_range in GX; eauto.
-    erewrite extends_same_length_stack in n. 2: eauto. omega.
+    rewrite mext_same_length0 in n; omega. 
    }
   apply extensionality; intros. unfold compose_meminj, inject_id.
   destruct (f x) as [[y delta] | ]; auto.
@@ -6546,8 +6562,10 @@ Qed.
 
 Lemma inject_extends_compose:
   forall f g m1 m2 m3,
-  inject f g m1 m2 -> extends m2 m3 -> inject f g m1 m3.
+    frameinj_surjective g (length (stack_adt m2)) ->
+    inject f g m1 m2 -> extends m2 m3 -> inject f g m1 m3.
 Proof.
+  intros f g m1 m2 m3 SURJ H H0.
   intros. inv H; inversion H0. constructor; intros.
 (* inj *)
   replace f with (compose_meminj f inject_id).
@@ -6589,11 +6607,11 @@ Proof.
   replace (flat_frameinj (length (stack_adt m1))) with
       (compose_frameinj (flat_frameinj (length (stack_adt m1))) (flat_frameinj (length (stack_adt m2)))).
   eapply mem_inj_compose; eauto.
+  rewrite mext_same_length0; apply surj_flat.
   {
     apply extensionality; intros. unfold compose_frameinj, flat_frameinj.
     destruct lt_dec; auto.
-    erewrite <- extends_same_length_stack; eauto.
-    destr.
+    rewrite mext_same_length0 in l; destr.
   }
   apply extensionality; intros. unfold compose_meminj, inject_id. auto.
   (* perm inv *)
@@ -6601,6 +6619,7 @@ Proof.
   eapply mext_perm_inv0; eauto.
   right; red; intros; elim A. eapply perm_extends; eauto.
   eapply inject_perm_condition_writable; constructor.
+  congruence.
 Qed.
 
 Remark flat_inj_no_overlap:
@@ -6682,6 +6701,7 @@ Proof.
   intros; red.
   exploit store_mapped_inj. eauto. eauto. apply flat_inj_no_overlap.
   unfold flat_inj. apply pred_dec_true; auto. eauto.
+  eauto.
   replace (ofs + 0) with ofs by omega.
   intros [m'' [A B]].
   erewrite store_stack_adt; eauto. congruence.
@@ -7173,11 +7193,15 @@ Proof.
   eapply H in l. 2: eauto. 2: eauto.  omega.
 Qed.
 
+
+Definition frameinj_surjective_after (g: frameinj) (s2: nat) (thr: nat) :=
+  forall j, thr <= j < s2 -> exists i, g i = Some j.
+
 Lemma frameinj_S_spec:
   forall g n1 n2
     (FPO: frameinj_preserves_order g)
     (RNG: forall i j : nat, g i = Some j -> i < n1 /\ j < n2)
-    (EX: forall j : nat, j < n2 -> exists i : nat, g i = Some j)
+    (EX: frameinj_surjective_after g n2 1)
     (PACK : forall i j : nat, g i = Some j -> j <= i),
   forall j i : nat, g (S i) = Some j -> forall j0, g i = Some j0 -> j = j0 \/ j = S j0.
 Proof.
@@ -7187,8 +7211,8 @@ Proof.
     exploit (FPO i (S i)); eauto. intro.
     destruct (Nat.eq_dec j0 (S j)); subst; auto.
     destruct (Nat.eq_dec (S j0) (S j)); subst; auto.
-    destruct (EX (S j0)).
-    eapply le_lt_trans with (S j).  omega. 
+    destruct (EX (S j0)). split. omega.
+    eapply le_lt_trans with (S j).  omega.
     eapply RNG. eauto.
     exploit (preserves_order_inv _ FPO j0 (S j0)). omega. eauto. eauto.
     exploit (preserves_order_inv _ FPO (S j0) (S j)). omega. eauto. eauto.
@@ -7199,17 +7223,12 @@ Lemma unrecord_stack_block_mem_inj_left:
   forall (m1 m1' m2 : mem) (j : meminj) g,
     mem_inj j g m1 m2 ->
     unrecord_stack_block m1 = Some m1' ->
-    (* (exists btop btop2 btop' delta1 delta2, *)
-    (*     is_stack_top (stack_adt m1) btop /\ *)
-    (*     is_stack_top (tl (stack_adt m1)) btop2 /\ *)
-    (*     j btop = Some (btop', delta1) /\ *)
-    (*     j btop2 = Some (btop', delta2) *)
-    (* ) -> *)
-    g 1 = Some 0 ->
+    (* frameinj_pack_after O g -> *)
+    (* frameinj_surjective_after g (length (stack_adt m2)) 1  -> *)
     (forall b, is_stack_top (stack_adt m1) b -> forall o k p, ~ Mem.perm m1 b o k p) ->
     mem_inj j (fun n => g (S n)) m1' m2.
 Proof.
-  intros m1 m1' m2 j g MI USB EXOTHERS TOPNOPERM.
+  intros m1 m1' m2 j g MI USB (* PACK EXOTHERS  *)TOPNOPERM.
   unfold_unrecord.
   inv MI; constructor; simpl; intros; eauto.
   eapply stack_inject_invariant_strong.
@@ -7234,25 +7253,24 @@ Proof.
       destruct GS; split; omega.
     + intros.
       destruct (stack_inject_exists_l (S i)); eauto. simpl; omega.
-    + intros.
-      destruct (stack_inject_exists_r j0); eauto.
-      destruct (Nat.eq_dec x O).
-      * subst.
-        assert (j0 = 0). apply stack_inject_pack in H1. omega. subst; exists 0; auto.
-      * destruct x. congruence. eauto. 
-    + generalize (frameinj_S_spec _ _ _ stack_inject_preserves_order stack_inject_range stack_inject_exists_r stack_inject_pack).
-      intros GSSpec.
-      induction i; simpl; intros; eauto.
-      specialize (GSSpec _ _ H0).
-      destruct (stack_inject_exists_l (S i)).
-      apply stack_inject_range in H0. intuition.
-      specialize (GSSpec _ H1). specialize (IHi _ H1).
-      destruct GSSpec; subst. eauto. omega.
+    (* + intros. *)
+    (*   destruct (stack_inject_exists_r j0); eauto. *)
+    (*   destruct (Nat.eq_dec x O). *)
+    (*   * subst. *)
+    (*     assert (j0 = 0). apply stack_inject_pack in H1. omega. subst; exists 0; auto. *)
+    (*   * destruct x. congruence. eauto.  *)
+    (* + generalize (frameinj_S_spec _ _ _ stack_inject_preserves_order stack_inject_range EXOTHERS). *)
+    (*   intros GSSpec. trim GSSpec. intros; eapply PACK; eauto. omega. *)
+    (*   induction i; simpl; intros; eauto. *)
+    (*   specialize (GSSpec _ _ H0). *)
+    (*   destruct (stack_inject_exists_l (S i)). *)
+    (*   apply stack_inject_range in H0. intuition. *)
+    (*   specialize (GSSpec _ H1). specialize (IHi _ H1). *)
+    (*   destruct GSSpec; subst. eauto. omega. *)
     + intros i1 i2 f1 f2 FAP1 FAP2 GS LT.
       eapply frame_at_pos_cons in FAP1. eapply stack_inject_sizes; eauto.
       intros i GI. destruct i. omega. apply Peano.le_n_S. apply LT. auto.
 Qed.
-
 
 Lemma frame_at_pos_cons_inv:
   forall a s i f,
@@ -7268,6 +7286,7 @@ Qed.
 Lemma unrecord_stack_block_mem_inj_parallel:
   forall (m1 m1' m2 : mem) (j : meminj) g
     (MINJ:  mem_inj j g m1 m2)
+    (PACK: frameinj_pack_after O g)
     (USB: unrecord_stack_block m1 = Some m1')
     (NO0: forall i j, g i = Some j -> O < i -> O < j),
     exists m2',
@@ -7315,7 +7334,7 @@ Proof.
       * generalize (stack_inject_compat _ _ _ JB 0 f). intro A. trim A.
         constructor; simpl; auto. trim A; auto.
         destruct A as (i2 & f2' & FAP & INF' & G0).
-        exploit stack_inject_pack. eauto. intros. assert (i2 = 0) by omega.
+        exploit PACK. 2: eauto. omega. intros. assert (i2 = 0) by omega.
         subst. inv FAP. simpl in H1. inv H1.
         exploit nodup_nodup'. apply stack_norepet. rewrite STK2.
         simpl; left; auto.
@@ -7330,18 +7349,18 @@ Proof.
       apply stack_inject_range in Heqo. simpl in *. omega.
     + intros.
       destruct (stack_inject_exists_l (S i)). simpl; omega. rewrite H1. simpl; eauto.
-    + intros.
-      destruct (stack_inject_exists_r (S j0)); eauto. simpl; omega.
-      destruct (Nat.eq_dec x O).
-      * subst.
-        exploit stack_inject_pack; eauto. intros. omega. 
-      * destruct x. congruence.
-        exists (x); rewrite H1. simpl. auto.
-    +
-      intros.
-      unfold option_map in H0. destr_in H0; inv H0.
-      exploit stack_inject_pack; eauto. simpl.
-      omega.
+    (* + intros. *)
+    (*   destruct (stack_inject_exists_r (S j0)); eauto. simpl; omega. *)
+    (*   destruct (Nat.eq_dec x O). *)
+    (*   * subst. *)
+    (*     exploit stack_inject_pack; eauto. intros. omega.  *)
+    (*   * destruct x. congruence. *)
+    (*     exists (x); rewrite H1. simpl. auto. *)
+    (* + *)
+    (*   intros. *)
+    (*   unfold option_map in H0. destr_in H0; inv H0. *)
+    (*   exploit stack_inject_pack; eauto. simpl. *)
+    (*   omega. *)
     + intros i1 i2 f1 f2 FAP1 FAP2 GS LT.
       unfold option_map in GS; destr_in GS; inv GS.
       eapply frame_at_pos_cons in FAP1.
@@ -7357,11 +7376,11 @@ Lemma unrecord_stack_block_inject_left:
   forall (m1 m1' m2 : mem) (j : meminj) g,
     inject j g m1 m2 ->
     unrecord_stack_block m1 = Some m1' ->
-    g 1 = Some 0 ->
+    (* g 1 = Some 0 -> *)
     (forall b, is_stack_top (stack_adt m1) b -> forall o k p, ~ Mem.perm m1 b o k p) ->
     inject j (fun n => g (S n)) m1' m2.
 Proof.
-  intros m1 m1' m2 j g INJ USB EXOTHERS NOPERM.
+  intros m1 m1' m2 j g INJ USB (* EXOTHERS  *)NOPERM.
   generalize (unrecord_stack_block_mem_unchanged _ _ USB). simpl. intros (NB & PERM & UNCH & LOAD).
   inv INJ; constructor; eauto.
   - eapply unrecord_stack_block_mem_inj_left; eauto. 
@@ -7376,12 +7395,13 @@ Lemma unrecord_stack_block_inject_parallel:
   forall (m1 m1' m2 : mem) (j : meminj) g,
     inject j g m1 m2 ->
     unrecord_stack_block m1 = Some m1' ->
+    frameinj_pack_after O g ->
     (forall i j0, g i = Some j0 -> 0 < i -> 0 < j0) ->
     exists m2',
       unrecord_stack_block m2 = Some m2' /\
       inject j (fun n => option_map pred (g (S n))) m1' m2'.
 Proof.
-  intros m1 m1' m2 j g INJ USB NOOTHER.
+  intros m1 m1' m2 j g INJ USB PACK NOOTHER.
   generalize (unrecord_stack_block_mem_unchanged _ _ USB). simpl. intros (NB & PERM & UNCH & LOAD).
   edestruct unrecord_stack_block_mem_inj_parallel as (m2' & USB' & MINJ); eauto. inv INJ; eauto.
   generalize (unrecord_stack_block_mem_unchanged _ _ USB'). simpl. intros (NB' & PERM' & UNCH' & LOAD').
@@ -7407,9 +7427,9 @@ Proof.
   - intros; rewrite <- ! EXT in *; eauto.
   - intros; rewrite <- ! EXT in *; eauto.
   - intros; rewrite <- ! EXT in *; eauto.
-  - intros. eapply stack_inject_exists_r in H; eauto. destruct H; eexists; eauto.
-    rewrite EXT in H; eauto. 
-  - intros; rewrite <- ! EXT in *; eauto.
+  (* - intros. eapply stack_inject_exists_r in H; eauto. destruct H; eexists; eauto. *)
+  (*   rewrite EXT in H; eauto.  *)
+  (* - intros; rewrite <- ! EXT in *; eauto. *)
   - intros; rewrite <- ! EXT in *; eauto.
     eapply stack_inject_sizes; eauto.
     intros; rewrite ! EXT in *; eauto.
@@ -7434,7 +7454,7 @@ Lemma unrecord_stack_block_extends:
         extends m1' m2'.
 Proof.
   intros.
-  exploit unrecord_stack_block_mem_inj_parallel. inv H; eauto. eauto.
+  exploit unrecord_stack_block_mem_inj_parallel. inv H; eauto. eauto. eauto.
   unfold flat_frameinj. intros i j A; destr_in A; inv A.
   intros (m2' & A & B).
   eexists; split; eauto.
@@ -7450,6 +7470,9 @@ Proof.
   destr. destr. omega. destr; omega.
   intros b ofs k p.
   rewrite ! Perm1. rewrite Perm2; auto.
+  revert mext_same_length0.
+  destruct (unrecord_stack_adt _ _ H0). rewrite H. simpl.
+  destruct (unrecord_stack_adt _ _ A). rewrite H1. simpl. auto.
 Qed.
 
 Lemma valid_frame_extends:
@@ -7466,11 +7489,14 @@ Qed.
 Lemma stack_inject_length_stack:
   forall j g P s1 s2,
     stack_inject j g P s1 s2 ->
+    frameinj_surjective g (length s2) ->
+    frameinj_pack_after O g ->
     length s2 <= length s1.
 Proof.
-  intros. inv H.
+  intros j g P s1 s2 SI SURJ PACK.
+  inv SI.
   destruct (Nat.eq_dec (length s2) 0). omega.
-  destruct (stack_inject_exists_r (length s2 - 1)).
+  destruct (SURJ (length s2 - 1)).
   omega.
   exploit stack_inject_range; eauto.
   intros (C & D).
@@ -7483,8 +7509,8 @@ Proof.
   intros.
   assert (x0 = length s2 - 1) by omega.
   subst.
-  apply stack_inject_pack in H0.
-  omega.
+  apply PACK in H0.
+  omega. omega.
 Qed.
 
 Lemma size_stack_pos:
@@ -7590,8 +7616,8 @@ Lemma size_stack_stack_inject:
 Proof.
   intros.
   transitivity (size_stack (map snd (filteri (fun i1 _ => latestb g i1 (length s1)) 0 s1))).
-  2: apply size_stack_filteri.
-  exploit stack_inject_length_stack; eauto. intro L.
+  2: apply size_stack_filteri. 
+  (* exploit stack_inject_length_stack; eauto. intro L. *)
   assert (list_forall2 (fun f1 f2 => frame_adt_size f1 = frame_adt_size f2) (map snd (filteri (fun i1 _ => latestb g i1 (length s1)) 0 s1)) s2).
   {
     admit.
@@ -7602,7 +7628,6 @@ Proof.
   induction 1; simpl; intros; eauto. omega.
   destruct b1, a1. destruct p, p0. simpl in H0; subst. omega.
 Admitted.
-
 
 Lemma size_stack_mem_inj:
   forall j g m1 m2,
@@ -7702,15 +7727,15 @@ Proof.
         apply stack_inject_range in Heqo. simpl; omega.
       * intros. destr. eauto. 
         edestruct stack_inject_exists_l; eauto. 2: rewrite H0.  simpl in H. omega.  simpl; eauto.
-      * intros. destruct (Nat.eq_dec j0 O); subst.
-        exists O; destr.
-        edestruct stack_inject_exists_r; eauto.
-        2: (exists (S x); simpl; rewrite H0).
-        instantiate (1:= pred j0). simpl in H; omega.
-        simpl. f_equal. omega.
-      * intros. destr_in H; inv H. omega.
-        unfold option_map in H1; destr_in H1. inv H1.
-        apply stack_inject_pack in Heqo. omega.
+      (* * intros. destruct (Nat.eq_dec j0 O); subst. *)
+      (*   exists O; destr. *)
+      (*   edestruct stack_inject_exists_r; eauto. *)
+      (*   2: (exists (S x); simpl; rewrite H0). *)
+      (*   instantiate (1:= pred j0). simpl in H; omega. *)
+      (*   simpl. f_equal. omega. *)
+      (* * intros. destr_in H; inv H. omega. *)
+      (*   unfold option_map in H1; destr_in H1. inv H1. *)
+      (*   apply stack_inject_pack in Heqo. omega. *)
       * intros. destr_in H1.
         -- subst. inv H. simpl in H3. inv H1. inv H3.
            inv H0. simpl in H; inv H. auto.
@@ -7734,14 +7759,15 @@ Qed.
 Lemma stack_inject_g0_0:
   forall j g p s1 s2,
     stack_inject j g p s1 s2 ->
+    frameinj_pack_after O g ->
     0 < length s1 ->
     0 < length s2 ->
     g 0 = Some 0.
 Proof.
-  intros j g p s1 s2 SI LT1 LT2.
+  intros j g p s1 s2 SI PACK LT1 LT2.
   inv SI.
-  destruct (stack_inject_exists_l _ LT1). rewrite H. apply stack_inject_pack in H. 
-  f_equal; omega.
+  destruct (stack_inject_exists_l _ LT1). rewrite H. apply PACK in H. 
+  f_equal; omega. omega.
 Qed.
 
 Lemma record_stack_blocks_mem_inj_left:
@@ -7751,15 +7777,16 @@ Lemma record_stack_blocks_mem_inj_left:
       frame_at_pos (stack_adt m2) O f2 ->
       frame_inject' j (perm m1) f1 f2 ->
       (forall b1 b2 delta, j b1 = Some (b2, delta) -> in_frame f1 b1 -> in_frame f2 b2) ->
-      g 0 = Some 0 ->
+      frameinj_pack_after O g ->
+      frameinj_surjective g (length (stack_adt m2)) ->
       mem_inj j (fun n => if Nat.eq_dec n 0 then Some 0 else g (pred n)) m1' m2.
 Proof.
-  intros j g m1 m2 f1 f2 m1' INJ ADT FAP FI INF G1; autospe.
+  intros j g m1 m2 f1 f2 m1' INJ ADT FAP FI INF G0 SURJ ; autospe.
   inv ADT.
   inversion INJ; subst; constructor; simpl; intros; eauto.
   eapply stack_inject_invariant_strong.
   intros. change (perm m1 b ofs k p) in H0. apply H0.
-  destruct mi_stack_blocks0.
+  inversion mi_stack_blocks0.
   constructor.
   - red; intros. destr_in H0. inv H0. omega.
     destr_in H1. omega. 
@@ -7782,14 +7809,19 @@ Proof.
   - intros. destr. eauto. 
     edestruct stack_inject_exists_l; eauto.  simpl in H.
     omega.
-  - intros. destruct (Nat.eq_dec j0 O); subst.
-    exists O; destr.
-    edestruct stack_inject_exists_r; eauto.
-    exists (S x); simpl; rewrite H0. auto.
-  - intros. destr_in H; inv H. omega.
-    apply stack_inject_pack in H1. omega.
+  (* - intros. destruct (Nat.eq_dec j0 O); subst. *)
+  (*   exists O; destr. *)
+  (*   edestruct stack_inject_exists_r; eauto. *)
+  (*   exists (S x); simpl; rewrite H0. auto. *)
+  (* - intros. destr_in H; inv H. omega. *)
+  (*   apply stack_inject_pack in H1. omega. *)
   - intros. destr_in H1.
-    + subst. inv H1. specialize (H2 1). trim H2. destr. omega.
+    + subst. inv H1. specialize (H2 1). trim H2. destr.
+      simpl. eapply stack_inject_g0_0. eauto. eauto.
+      exploit stack_inject_length_stack. eauto. eauto. eauto.
+      apply frame_at_pos_lt in H0. omega.
+      apply frame_at_pos_lt in H0. omega.
+      omega.
     + apply frame_at_pos_cons_inv in H; try omega.
       eapply stack_inject_sizes; eauto.
       intros. specialize (H2 (S i)). destr_in H2. simpl in H2. trim H2; auto. omega.
@@ -7856,6 +7888,8 @@ Proof.
     destr. omega. destr. destr. simpl. f_equal. omega. omega.
     destr. omega.
     rewrite ! PERM1, PERM in *. eauto.
+    rewrite (record_stack_blocks_stack_adt _ _ _ ADT).
+    rewrite (record_stack_blocks_stack_adt _ _ _ ADT'). simpl; congruence.
 Qed.
 
 Lemma free_list_stack_blocks:
@@ -7914,7 +7948,9 @@ Lemma record_stack_block_inject_left:
      (INJ: inject j g m1 m2)
      (FAP: frame_at_pos (stack_adt m2) 0 f2)
      (FI: frame_inject' j (perm m1) f1 f2)
-     (RSB: record_stack_blocks m1 f1 m1'),
+     (RSB: record_stack_blocks m1 f1 m1')
+     (FPA: frameinj_pack_after O g)
+     (SURJ: frameinj_surjective g (length (stack_adt m2))),
      inject j (fun n : nat => if Nat.eq_dec n 0 then Some 0 else g (Init.Nat.pred n)) m1' m2.
 Proof.
   intros.
@@ -7922,10 +7958,6 @@ Proof.
   exploit record_stack_blocks_mem_inj_left; eauto.
   - intros. inv FI. rewrite Forall_forall in frame_inject_inj.
     eapply frame_inject_inj; eauto.
-  - inv mi_inj0.
-    exploit stack_inject_length_stack. eauto. intros.
-    exploit frame_at_pos_lt; eauto. intro LT.
-    eapply stack_inject_g0_0; eauto. omega.
   - intro MINJ.
     edestruct (record_stack_blocks_mem_unchanged _ _ _ RSB) as (NB1 & PERM1 & U1 & C1) ; simpl in *.
     inversion INJ; econstructor; simpl; intros; eauto.
@@ -8021,7 +8053,7 @@ Lemma unrecord_stack_block_inject_neutral:
     inject_neutral thr m'.
 Proof.
   intros.
-  exploit unrecord_stack_block_mem_inj_parallel. eauto. eauto.
+  exploit unrecord_stack_block_mem_inj_parallel. eauto. eauto. eauto.
   unfold flat_frameinj. intros. destr_in H1.
   intros (m2' & RSB & MI). rewrite H0 in RSB; inv RSB.
   eapply mem_inj_frame_inj_ext; eauto.
